
%
%  $Description: Author guidelines and sample document in LaTeX 2.09$ 
%
%  $Author: ienne $
%  $Date: 1995/09/15 15:20:59 $
%  $Revision: 1.4 $
%

\documentclass[times, 10pt,twocolumn]{article} 
\usepackage{paper}
\usepackage{times}
\usepackage{graphicx}
\usepackage{float}
\usepackage{amsmath}

%\documentstyle[times,art10,twocolumn,latex8]{article}

%------------------------------------------------------------------------- 
% take the % away on next line to produce the final camera-ready version 
\pagestyle{empty}

%------------------------------------------------------------------------- 
\begin{document}

\title{18-752 Final Project Report: EMG Signal Classification}

\author{Paul Griffioen\\Dept. of Electrical and Computer Engineering\\Carnegie Mellon University\\ pgriffi1@andrew.cmu.edu\\
% For a paper whose authors are all at the same institution, 
% omit the following lines up until the closing ``}''.
% Additional authors and addresses can be added with ``\and'', 
% just like the second author.
\and
Thomas Mayo-Smith\\Dept. of Electrical and Computer Engineering\\Carnegie Mellon University\\tmayosmi@andrew.cmu.edu\\
}

\maketitle
\thispagestyle{empty}

%------------------------------------------------------------------------- 
\begin{abstract}
Abstract.
\end{abstract}

%------------------------------------------------------------------------- 
\section{Introduction and Motivation}

Introduction and motivation.

%------------------------------------------------------------------------- 
\section{Data Set Collection}

Data set collection.

%------------------------------------------------------------------------- 
\section{Blind Identification and Detection}

Blind identification and detection.

\begin{equation}
x = \text{EMG sample}
\end{equation}
\begin{equation}
\lambda_i = \text{contraction }i, i\in[1,2,3,4]
\end{equation}
\begin{equation}
f_{\theta_i}(x|\lambda_i) = \theta_i\mathrm{e}^{-\theta_ix}
\end{equation}
\begin{equation}
f_{\theta_i}(\lambda_i) = (\text{\# data points for }\lambda_i)/(\text{total \# of labeled data points})
\end{equation}
\begin{equation}
L(\theta_i,\lambda_i,X) = \log{f_{\theta_i}(X|\lambda_i)} = \log{\prod_{k=1}^{n}f_{\theta_i}(x_k|\lambda_i)} = \sum_{k=1}^{n}\log{f_{\theta_i}(x_k|\lambda_i)}
\end{equation}
\begin{equation}
\frac{\partial}{\partial{\theta_i}}L(\theta_i,\lambda_i,X) = 0 \text{ } => \text{ } \hat{\theta}_i = \frac{n}{\sum_{k=1}^{n}x_k}
\end{equation}
\begin{equation}
f_{\theta_i}(\lambda_i|x) = \frac{f_{\theta_i}(\lambda_i)\prod_{\text{channel}}f_{\theta_i}(x|\lambda_i)}{\sum_{i=1}^{4}f_{\theta_i}(\lambda_i)\prod_{\text{channel}}f_{\theta_i}(x|\lambda_i)}
\end{equation}
\begin{equation}
\hat{\lambda} = \max_{i}f_{\theta_i}(\lambda_i|x)
\end{equation}

%------------------------------------------------------------------------- 
\section{Supervised Identification and Detection}

Supervised Identification and Detection.

\begin{equation}
x = \text{EMG sample}
\end{equation}
\begin{equation}
\lambda_i = \text{contraction }i, i\in[1,2,3,4]
\end{equation}
\begin{equation}
f_{\mu_i,\sigma_i^2}(x|\lambda_i) = \mathcal{N}(\mu_i,\sigma_i^2)
\end{equation}
\begin{equation}
f_{\mu_i,\sigma_i^2}(\lambda_i) = \text{categorical density with parameters } p_i
\end{equation}
\begin{equation}
f(x) = \sum_{i=1}^{4}f_{\mu_i,\sigma_i^2}(\lambda_i)f_{\mu_i,\sigma_i^2}(x|\lambda_i)
\end{equation}
\begin{equation}
L(\mu,\sigma^2,\lambda,X) = \log{f_{\mu,\sigma^2}(X)} = \sum_{k=1}^{n}\log{\sum_{i=1}^{4}f_{\mu_i,\sigma_i^2}(x_k|\lambda_i)f_{\mu_i,\sigma_i^2}(\lambda_i)}
\end{equation}
\begin{equation}
\frac{\partial}{\partial{\mu}}L(\mu,\sigma^2,\lambda,X) = 0 \text{ } => \text{ } \hat{\mu}
\end{equation}
\begin{equation}
\frac{\partial}{\partial{\sigma^2}}L(\mu,\sigma^2,\lambda,X) = 0 \text{ } => \text{ } \hat{\sigma}^2
\end{equation}
\begin{equation}
\text{calculate } f_{\hat{\mu}_i,\hat{\sigma}_i^2}(\lambda_i|x_k)
\end{equation}
\begin{equation}
f_{\mu_i,\sigma_i^2}(\lambda_i|x) = \frac{1}{n}\sum_{k=1}^{n}f_{\hat{\mu}_i,\hat{\sigma}_i^2}(\lambda_i|x_k)
\mu_i = \frac{\sum_{k=1}^{n}f_{\hat{\mu}_i,\hat{\sigma}_i^2}(\lambda_i|x_k)x_k}{\sum_{k=1}^{n}f_{\hat{\mu}_i,\hat{\sigma}_i^2}(\lambda_i|x_k)}
\end{equation}
\begin{equation}
\sigma_i^2 = \frac{\sum_{k=1}^{n}f_{\hat{\mu}_i,\hat{\sigma}_i^2}(\lambda_i|x_k)(x_k-\mu_i)(x_k-\mu_i)^T}{\sum_{k=1}^{n}f_{\hat{\mu}_i,\hat{\sigma}_i^2}(\lambda_i|x_k)}
\end{equation}

%------------------------------------------------------------------------- 
\nocite{ex1,ex2}
\bibliographystyle{paper}
\bibliography{paper}

%\begin{thebibliography}{}
\begin{thebibliography}{}\setlength{\itemsep}{-1ex}\small

\bibitem{incentives}
Author. "Title." \textit{Journal}, pp. \#-\#, Year.

\end{thebibliography}

\end{document}
